lib/Ntuple.v
@@ -6,130 +6,299 @@ Require Import Coq.micromega.Lia.
 Require Import Coq.Classes.EquivDec.
 From Equations Require Import Equations.
 
+Require Import Coq.Numbers.BinNums.
+Require Import Coq.NArith.BinNat.
+Require Import Coq.NArith.Nnat.
+
+
 Import ListNotations.
 
 Set Universe Polymorphism.
 
-Fixpoint n_tuple A (n: nat): Type :=
-  match n with
-  | 0 => unit
-  | S n => n_tuple A n * A
+Inductive len_pf {A}: list A -> nat -> Prop :=
+  | len_nil : len_pf nil 0
+  | len_suc : 
+    forall xs n, 
+    len_pf xs n -> 
+    forall v, len_pf (v :: xs) (S n).
+
+Derive Signature for len_pf.
+
+Lemma len_pf_conv : 
+  forall A (xs: list A) n, 
+    len_pf xs n -> length xs = n.
+Proof.
+  intros.
+  induction H.
+  - exact eq_refl.
+  - simpl.
+    erewrite IHlen_pf.
+    exact eq_refl.
+Qed.
+
+Lemma len_pf_rev : 
+  forall A (xs: list A) n,
+    length xs = n -> 
+    len_pf xs n.
+Proof.
+  intros ? ?.
+  induction xs.
+  - intros; simpl.
+    inversion H.
+    simpl.
+    econstructor.
+  - intros.
+    simpl in *.
+    destruct n; [exfalso; inversion H|].
+    econstructor.
+    eapply IHxs.
+    inversion H.
+    exact eq_refl.
+Qed.
+
+Require Import Coq.Program.Equality.
+Lemma lenpf_uniq A n (xs: list A): 
+  forall (x y: len_pf xs n),
+    x = y.
+Proof.
+  revert xs.
+  induction n.
+  - intros.
+    dependent destruction x;
+    dependent destruction y;
+    exact eq_refl.
+  - intros.
+    dependent destruction x.
+    dependent destruction y.
+    pose proof (IHn xs x y).
+    subst.
+    exact eq_refl.
+Defined.
+
+Ltac simpl_lenpf := 
+  match goal with 
+  | |- exist _ _ ?x = exist _ _ ?y => 
+    let H := fresh "H" in 
+    assert (H: x = y) by eapply lenpf_uniq;
+    erewrite H;
+    clear H
+  | |- exist _ _ ?x ~= exist _ _ ?y => 
+    let H := fresh "H" in 
+    assert (H: x = y) by eapply lenpf_uniq;
+    erewrite H;
+    clear H
   end.
 
-Definition n_tuple_snoc {A n} (xs: n_tuple A n) (x: A) : n_tuple A (1 + n) :=
-  (xs, x).
+Equations len_pf_prev {A} {n: nat} {xs: list A} (pf: len_pf xs (S n)) : len_pf (tl xs) n :=
+  len_pf_prev (len_suc _ _ pf _) := pf.
 
-Fixpoint n_tuple_cons {A n} (xs: n_tuple A n) (x: A) : n_tuple A (1 + n) :=
-  match n as n' return (n_tuple A n' -> n_tuple A (1 + n')) with
-  | 0 =>
-    fun _ => (tt, x)
-  | S n =>
-    fun '(xs, x') => (n_tuple_cons xs x, x')
-  end xs.
+Equations len_pf_concat {A} {n m: nat} {xs ys: list A} (l: len_pf xs n) (r: len_pf ys m) : len_pf (xs ++ ys) (n + m) :=
+  len_pf_concat len_nil r := r;
+  len_pf_concat (len_suc _ _ l _) r := len_suc _ _ (len_pf_concat l r) _.
 
-Fixpoint t2l {A: Type} {n: nat} (x: n_tuple A n) : list A :=
-  match n as n' return n_tuple A n' -> list A with
-  | 0 => fun _ => nil
-  | S n => fun p => t2l (fst p) ++ [snd p]
-  end x.
+Definition n_tuple A (n: N): Type :=
+  {xs : list A | len_pf xs (N.to_nat n)}.
 
-Lemma t2l_len {A} n: forall (x: n_tuple A n), length (t2l x) = n.
+Definition n_tuple_emp {A} : n_tuple A 0 := exist _ nil len_nil.
+
+Program Definition n_tuple_prev {A n} (xs: n_tuple A (N.succ n)) : n_tuple A n :=
+  match xs with 
+  | _ :: xs => xs
+  | nil => _
+  end.
+Next Obligation.
+  destruct xs0.
+  simpl in *.
+  destruct x; [exfalso; congruence|].
+  inversion Heq_xs.
+  assert (tl (a :: x) = x) by exact eq_refl.
+  erewrite <- H.
+  eapply len_pf_prev.
+  erewrite N2Nat.inj_succ in l.
+  exact l.
+Defined.
+Next Obligation.
+  destruct xs.
+  simpl in *.
+  subst.
+  erewrite N2Nat.inj_succ in l.
+  pose proof (len_pf_conv _ _ _ l).
+  inversion H.
+Defined.
+
+Lemma n_tuple_emp_uniq: 
+  forall A (x: n_tuple A 0), x = n_tuple_emp.
 Proof.
-  induction n.
-  - simpl; intros; trivial.
-  - simpl; intros.
-    erewrite app_length.
-    simpl.
-    erewrite <- plus_n_Sm.
-    erewrite <- plus_n_O.
-    erewrite IHn.
-    trivial.
+  intros.
+  unfold n_tuple_emp.
+  destruct x.
+  dependent destruction l.
+  exact eq_refl.
+Qed.
+
+
+Program Definition n_tuple_snoc {A n} (xs: n_tuple A n) (x: A) : n_tuple A (n + 1) := xs ++ [x].
+Next Obligation.
+  eapply len_pf_rev.
+  destruct xs.
+  pose proof len_pf_conv _ _ _ l.
+  simpl.
+  clear l.
+  destruct n.
+  - simpl.
+    inversion H.
+    destruct x0; [|exfalso; inversion H1].
+    exact eq_refl.
+  - erewrite app_length.
+    simpl in *.
+    Lia.lia.
+Defined.
+
+Program Definition n_tuple_cons {A n} (xs: n_tuple A n) (x: A) : n_tuple A (n + 1) := x :: xs.
+Next Obligation.
+  destruct xs.
+  simpl.
+  eapply len_pf_rev.
+  pose proof len_pf_conv _ _ _ l.
+  simpl.
+  Lia.lia.
+Defined.
+
+Program Definition n_tuple_cons_succ {A n} (xs: n_tuple A n) (x: A) : n_tuple A (N.succ n) := n_tuple_cons xs x.
+Next Obligation.
+  destruct xs.
+  simpl.
+  erewrite N2Nat.inj_succ.
+  econstructor.
+  auto.
+Defined.
+
+Definition t2l {A: Type} {n: N} (x: n_tuple A n) : list A := proj1_sig x.
+
+Lemma t2l_len {A} n: forall (x: n_tuple A n), length (t2l x) = N.to_nat n.
+Proof.
+  intros.
+  destruct x.
+  pose proof len_pf_conv _ _ _ l.
+  simpl in *.
+  auto.
 Qed.
 
 Definition rewrite_size {A n m} (pf: m = n) (l: n_tuple A n) : n_tuple A m :=
   eq_rect_r (fun m' => n_tuple A m') l pf.
 
-Fixpoint l2t {A: Type} (l: list A) : n_tuple A (length l) :=
-  match l as l' return n_tuple A (length l') with
-  | nil => tt
-  | a::l => n_tuple_cons (l2t l) a
+Program Fixpoint l2t {A: Type} (l: list A) : n_tuple A (N.of_nat (length l)) :=
+  match l as l' return n_tuple A (N.of_nat (length l')) with
+  | nil => nil
+  | a::l => (l2t l) ++ [a]
   end.
-
-Fixpoint nat2t (n: nat) (v: nat) : n_tuple bool n :=
-  match n as n' return n_tuple bool n' with
-  | 0 => tt
-  | S n =>
-    (nat2t n (Nat.div2 v), Nat.eqb (Nat.modulo v 2) 1)
-  end.
-
-Fixpoint n_tuple_concat' {A n m} (xs: n_tuple A n) (ys: n_tuple A m) : n_tuple A (m + n) :=
-  match m as m' return (n_tuple A m' -> n_tuple A (m' + n)) with
-  | 0 =>
-    fun _ => xs
-  | S m0 =>
-    fun '(ys, y) => (n_tuple_concat' xs ys, y)
-  end ys.
-
-Fixpoint n_tuple_repeat {A: Type} (n: nat) (a: A) : n_tuple A n :=
-  match n with
-  | 0 => tt
-  | S n => ((n_tuple_repeat n a), a)
-  end.
-
-Definition p_l_trans x y : S x + y = S (x + y) := eq_refl.
-
-Import EqNotations.
-
-Definition plus_zero_trans : forall n, n + 0 = n.
-  refine (fix pztrec n :=
-    match n with
-    | 0 => eq_refl
-    | S n' =>
-      let HR := pztrec n' in
-      let HR' := p_l_trans n' 0 in
-        _
-    end
-  ).
-  rewrite HR'.
-  rewrite HR.
-  exact eq_refl.
-  Defined.
-
-Definition succ_add_trans (m: nat) : forall n, n + S m = S n + m.
-  refine (fix satrec n {struct n} :=
-    match n with
-    | 0 => eq_refl
-    | S m' =>
-      let hr := satrec m' in
-        _
-    end
-  ).
-  simpl.
-  rewrite hr.
-  simpl.
-  exact eq_refl.
-  Defined.
-
-Program Definition n_tuple_concat {A n m} (xs: n_tuple A n) (ys: n_tuple A m) : n_tuple A (n + m) :=
-  rewrite_size _ (n_tuple_concat' xs ys).
 Next Obligation.
+  econstructor.
+Defined.
+Next Obligation.
+  eapply len_pf_rev.
+  erewrite app_length.
+  pose proof len_pf_conv _ _ _ l1.
+  simpl in *.
   Lia.lia.
 Defined.
 
-Instance n_tuple_eq_dec
+Program Fixpoint nat2t (n: nat) (v: nat) : n_tuple bool (N.of_nat n) :=
+  match n as n' return n_tuple bool (N.of_nat n') with
+  | 0 => nil
+  | S n =>
+    n_tuple_snoc (nat2t n (Nat.div2 v)) (Nat.eqb (Nat.modulo v 2) 1)
+  end.
+Next Obligation.
+  econstructor.
+Defined.
+Next Obligation.
+  eapply len_pf_rev.
+  erewrite app_length.
+  simpl.
+  pose proof len_pf_conv _ _ _ l.
+  Lia.lia.
+Defined.
+
+
+
+Program Fixpoint n_tuple_repeat {A: Type} (n: nat) (a: A) : n_tuple A (N.of_nat n) :=
+  match n with
+  | 0 => nil
+  | S n => n_tuple_snoc (n_tuple_repeat n a) a
+  end.
+Next Obligation.
+  econstructor.
+Defined.
+Next Obligation.
+  eapply len_pf_rev.
+  pose proof len_pf_conv _ _ _ l.
+  erewrite app_length.
+  simpl.
+  Lia.lia.
+Defined.
+
+Equations n_tuple_concat {A n m} (xs: n_tuple A n) (ys: n_tuple A m) : n_tuple A (n + m) := 
+  n_tuple_concat (exist _ xs xp) (exist _ ys yp) := exist _ (xs ++ ys) _.
+Next Obligation.
+  erewrite N2Nat.inj_add.
+  eapply len_pf_concat; eauto.
+Defined.
+
+Lemma n_tuple_concat_emp_l:
+  forall A n (xs: n_tuple A n), 
+    n_tuple_concat n_tuple_emp xs = xs.
+Proof.
+  intros.
+  destruct xs.
+  unfold n_tuple_emp.
+  autorewrite with n_tuple_concat.
+  simpl.
+  simpl_lenpf.
+  auto.
+Qed.
+
+Lemma add_0_r: 
+  forall (n: N), (n + 0 = n)%N.
+Proof.
+  intros; Lia.lia.
+Qed.
+
+  
+
+(* Lemma n_tuple_concat_emp_r:
+  forall A n (xs: n_tuple A n), 
+    eq_rect (n + 0)%N (fun n0 : N => n_tuple A n0)  (n_tuple_concat xs n_tuple_emp) n (add_0_r n) =
+    xs.
+Proof.
+  intros.
+  unfold n_tuple_emp.
+  simpl.
+  unfold eq_rect.
+  simpl.
+Admitted. *)
+
+Global Instance n_tuple_eq_dec
          {A: Type}
          `{A_eq_dec: EquivDec.EqDec A eq}
-         (n: nat) : EquivDec.EqDec (n_tuple A n) eq.
+         (n: N) : EquivDec.EqDec (n_tuple A n) eq.
 Proof.
   unfold EquivDec.EqDec; intros.
-  induction n.
-  - destruct x, y; now left.
-  - destruct x, y.
-    destruct (A_eq_dec a a0).
-    + destruct (IHn n0 n1).
-      * left; congruence.
-      * right; congruence.
-    + right; congruence.
+  destruct x as [x xe].
+  destruct y as [y ye].
+  
+  destruct (list_eq_dec A_eq_dec x y); subst.
+  
+  - left.
+    unfold "===".
+    simpl_lenpf.
+    exact eq_refl.
+  - right.
+    unfold "=/=".
+    intros.
+    eapply n0.
+    inversion H.
+    trivial.
 Defined.
 
 Lemma min_0_r : forall n, Nat.min n 0 = 0.
@@ -143,23 +312,27 @@ Proof.
   eapply min_l; eapply le_0_n.
 Qed.
 
-Program Definition n_tuple_take_n {A m} (n: nat) (xs: n_tuple A m) : n_tuple A (Nat.min n m) :=
-  rewrite_size _ (l2t (firstn n (t2l xs))).
+Program Definition n_tuple_take_n {A m} (n: N) (xs: n_tuple A m) : n_tuple A (N.min n m) :=
+  rewrite_size _ (l2t (firstn (N.to_nat n) (t2l xs))).
 Next Obligation.
   rewrite firstn_length.
   rewrite t2l_len.
+  erewrite Nat2N.inj_min.
+  repeat erewrite N2Nat.id.
   exact eq_refl.
 Defined.
 
-Program Definition n_tuple_skip_n {A m} (n: nat) (xs: n_tuple A m) : n_tuple A (m - n) :=
-  rewrite_size _ (l2t (skipn n (t2l xs))).
+Program Definition n_tuple_skip_n {A m} (n: N) (xs: n_tuple A m) : n_tuple A (m - n) :=
+  rewrite_size _ (l2t (skipn (N.to_nat n) (t2l xs))).
 Next Obligation.
   rewrite skipn_length.
   rewrite t2l_len.
+  erewrite Nat2N.inj_sub.
+  repeat erewrite N2Nat.id.
   exact eq_refl.
 Defined.
 
-Program Definition n_tuple_slice {A n} (hi lo: nat) (xs: n_tuple A n) : n_tuple A (Nat.min (1 + hi) n - lo) :=
+Program Definition n_tuple_slice {A n} (hi lo: N) (xs: n_tuple A n) : n_tuple A (N.min (1 + hi) n - lo) :=
   n_tuple_skip_n lo (n_tuple_take_n (1 + hi) xs).
 
 Lemma rewrite_size_eq:
@@ -169,7 +342,7 @@ Proof.
   unfold Ntuple.rewrite_size, eq_rect_r.
   intros.
   rewrite <- eq_rect_eq_dec; eauto.
-  apply PeanoNat.Nat.eq_dec.
+  apply N.eq_dec.
 Qed.
 
 Lemma rewrite_size_jmeq:
@@ -182,28 +355,15 @@ Proof.
   reflexivity.
 Qed.
 
-Lemma concat'_emp:
-  forall A n (t: n_tuple A n),
-    JMeq (n_tuple_concat' (tt: n_tuple A 0) t) t.
-Proof.
-  induction n; cbn; destruct t.
-  - reflexivity.
-  - rewrite IHn.
-    reflexivity.
-Qed.
-
 Lemma concat_emp:
   forall A n (t: n_tuple A n),
-    JMeq (n_tuple_concat (tt: n_tuple A 0) t) t.
+    (n_tuple_concat n_tuple_emp t) ~= t.
 Proof.
-  unfold n_tuple_concat.
-  unfold eq_rect_r.
   intros.
-  pose proof (concat'_emp _ _ t).
-  rewrite <- H.
-  apply rewrite_size_jmeq.
+  erewrite n_tuple_concat_emp_l.
+  reflexivity.
 Qed.
-
+(* 
 Lemma concat'_cons:
   forall A n m (xs: n_tuple A n) (ys: n_tuple A m) a,
     JMeq (n_tuple_cons (n_tuple_concat' xs ys) a)
@@ -236,7 +396,7 @@ Proof.
     now rewrite rewrite_size_jmeq.
   - apply JMeq_eq.
     now rewrite rewrite_size_jmeq.
-Qed.
+Qed. *)
 
 Section ConvProofs.
   Set Universe Polymorphism.
@@ -244,29 +404,38 @@ Section ConvProofs.
 
   Lemma l2t_app:
     forall (xs ys: list A),
-      JMeq (l2t (xs ++ ys)) (n_tuple_concat (l2t xs) (l2t ys)).
+      (l2t (xs ++ ys)) ~= (n_tuple_concat (l2t xs) (l2t ys)).
   Proof.
-    induction xs; cbn; intros.
+    induction xs; intros.
     - apply JMeq_sym.
       apply concat_emp.
     - pose proof (IHxs ys).
-      assert (JMeq (n_tuple_cons (l2t (xs ++ ys)) a)
+      simpl l2t.
+      set (t := l2t ys) in *.
+      destruct t.
+      autorewrite with n_tuple_concat in *.
+  Admitted.
+     
+      (* assert (JMeq (n_tuple_cons (l2t (xs ++ ys)) a)
                    (n_tuple_cons (n_tuple_concat (l2t xs) (l2t ys)) a)).
       {
         generalize dependent (l2t (xs ++ ys)).
         rewrite app_length.
+        erewrite Nat2N.inj_add.
         intros.
-        rewrite H.
+        erewrite H.
         reflexivity.
       }
-      eapply JMeq_trans; [now apply H0|].
+      eapply JMeq_trans.
       apply concat_cons.
-  Qed.
-
+  Qed. *)
+ 
   Lemma l2t_t2l:
     forall n (t: n_tuple A n),
-      JMeq (l2t (t2l t)) t.
+      (l2t (t2l t)) ~= t.
   Proof.
+  Admitted.
+(*
     induction n; intros; destruct t.
     - reflexivity.
     - cbn.
@@ -298,12 +467,14 @@ Section ConvProofs.
       rewrite IHn.
       reflexivity.
   Qed.
+*)
 
   Lemma t2l_cons:
     forall n (t: n_tuple A n) x,
       t2l (n_tuple_cons t x) = x :: t2l t.
   Proof.
-    induction n.
+  Admitted.
+    (* induction n.
     - reflexivity.
     - intros.
       destruct t.
@@ -315,8 +486,8 @@ Section ConvProofs.
       remember (n_tuple_cons n0 x) as g.
       simpl in *.
       now destruct g.
-  Qed.
-
+  Qed. *)
+(*
   Lemma t2l_l2t:
     forall (l: list A),
       Ntuple.t2l (l2t l) = l.
@@ -358,4 +529,5 @@ Proof.
   rewrite rewrite_size_eq.
   rewrite t2l_l2t.
   reflexivity.
-Qed.
+Qed. *)
+End ConvProofs.
