lib/Bisimulations/Leaps.v
@@ -7,15 +7,21 @@ Require Import Leapfrog.FinType.
 Require Import Leapfrog.ConfRel.
 Require Import Leapfrog.Relations.
 Require Leapfrog.Bisimulations.Semantic.
+
+Require Import Coq.Numbers.BinNums.
+Require Import Coq.NArith.BinNat.
+Require Import Coq.NArith.Nnat.
+
 Module BS := Leapfrog.Bisimulations.Semantic.
+
 
 Section Leaps.
   Variable (a: p4automaton).
   Notation conf := (configuration a).
 
-  Definition leap_size (q1 q2: conf) : nat :=
+  Definition leap_size (q1 q2: conf) : N :=
     match conf_state q1, conf_state q2 with
-    | inl s1, inl s2 => min (configuration_room_left q1) (configuration_room_left q2)
+    | inl s1, inl s2 => N.min (configuration_room_left q1) (configuration_room_left q2)
     | inl s1, inr _ => configuration_room_left q1
     | inr _, inl s2 => configuration_room_left q2
     | inr _, inr _ => 1
@@ -30,7 +36,7 @@ Section Leaps.
         (b: bool):
         close_interpolate R q1 q2 ->
         (forall buf,
-            length buf = leap_size q1 q2 ->
+            (N.of_nat (length buf)) = leap_size q1 q2 ->
             R (follow q1 buf) (follow q2 buf)) ->
         close_interpolate R (step q1 b) (step q2 b).
 
@@ -39,7 +45,7 @@ Section Leaps.
       forall q1 q2,
         (accepting q1 <-> accepting q2) ->
         (forall buf,
-          length buf = leap_size q1 q2 ->
+          (N.of_nat (length buf)) = leap_size q1 q2 ->
           bisimilar_with_leaps (follow q1 buf) (follow q2 buf)) ->
         bisimilar_with_leaps q1 q2.
 
