lib/Bisimulations/Syntactic.v
@@ -8,6 +8,10 @@ Require Import Leapfrog.Ntuple.
 
 Require Leapfrog.Bisimulations.Semantic.
 
+Require Import Coq.Numbers.BinNums.
+Require Import Coq.NArith.BinNat.
+Require Import Coq.NArith.Nnat.
+
 Section Syntactic.
   Variable (St1: Type).
   Context `{St1_eq_dec: EquivDec.EqDec St1 eq}.
@@ -19,12 +23,12 @@ Section Syntactic.
 
   (* Header identifiers. *)
   Variable (Hdr1: Type).
-  Variable (Hdr1_sz : Hdr1 -> nat).
+  Variable (Hdr1_sz : Hdr1 -> N).
   Context `{Hdr1_eq_dec: EquivDec.EqDec Hdr1 eq}.
   Context `{Hdr1_finite: @Finite Hdr1 _ Hdr1_eq_dec}.
 
   Variable (Hdr2: Type).
-  Variable (Hdr2_sz : Hdr2 -> nat).
+  Variable (Hdr2_sz : Hdr2 -> N).
   Context `{Hdr2_eq_dec: EquivDec.EqDec Hdr2 eq}.
   Context `{Hdr2_finite: @Finite Hdr2 _ Hdr2_eq_dec}.
 
