lib/FirstOrderConfRelSimplified.v
@@ -11,6 +11,10 @@ Import ListNotations.
 Import HListNotations.
 Local Open Scope program_scope.
 
+Require Import Coq.Numbers.BinNums.
+Require Import Coq.NArith.BinNat.
+Require Import Coq.NArith.Nnat.
+
 Set Universe Polymorphism.
 
 Section AutModel.
@@ -24,19 +28,19 @@ Section AutModel.
   Variable (Hdr: Type).
   Context `{Hdr_eq_dec: EquivDec.EqDec Hdr eq}.
   Context `{Hdr_finite: @Finite Hdr _ Hdr_eq_dec}.
-  Variable (Hdr_sz: Hdr -> nat).
+  Variable (Hdr_sz: Hdr -> N).
 
   Variable (a: P4A.t St Hdr_sz).
 
   Inductive sorts: Type :=
-  | Bits (n: nat)
+  | Bits (n: N)
   | Store.
   Derive NoConfusion for sorts.
 
   Inductive funs: arity sorts -> sorts -> Type :=
   | BitsLit: forall n, n_tuple bool n -> funs [] (Bits n)
   | Concat: forall n m, funs [Bits n; Bits m] (Bits (n + m))
-  | Slice: forall n hi lo, funs [Bits n] (Bits (Nat.min (1 + hi) n - lo))
+  | Slice: forall n hi lo, funs [Bits n] (Bits (N.min (1 + hi) n - lo))
   | Lookup: forall h, funs [Store] (Bits (Hdr_sz h)).
 
   Inductive rels: arity sorts -> Type :=.
@@ -61,14 +65,14 @@ Section AutModel.
              (f: sig_funs sig params ret)
              (args: HList.t mod_sorts params)
     : mod_sorts ret :=
-    { mod_fns (BitsLit n xs) hnil := xs;
+    { mod_fns (BitsLit xs) hnil := xs;
       mod_fns (Concat n m) (xs ::: ys ::: hnil) :=
         n_tuple_concat xs ys;
       mod_fns (Slice n hi lo) (xs ::: hnil) :=
         n_tuple_slice hi lo xs;
       mod_fns (Lookup k) (store ::: hnil) :=
         match P4A.find Hdr Hdr_sz k store with
-        | P4A.VBits _ v => v
+        | P4A.VBits v => v
         end
     }.
 
@@ -85,7 +89,9 @@ Section AutModel.
   |}.
 
   Obligation Tactic := intros.
-  Equations simplify_concat_zero {ctx srt} (e: tm ctx srt) : tm ctx srt :=
+  Definition simplify_concat_zero {ctx srt} (e: tm ctx srt) : tm ctx srt.
+  Admitted.
+  (* Equations simplify_concat_zero {ctx srt} (e: tm ctx srt) : tm ctx srt :=
     { simplify_concat_zero (TFun sig (Concat 0 m) (_ ::: x ::: hnil)) :=
         simplify_concat_zero x;
       simplify_concat_zero (TFun sig (Concat (S n) m) (x ::: y ::: hnil)) :=
@@ -97,12 +103,14 @@ Section AutModel.
       simplify_concat_zero (TFun sig f args) :=
         TFun sig f args;
       simplify_concat_zero (TVar x) := TVar x;
-    }.
+    }. *)
+
+  
 
   Import Coq.Program.Equality.
 
   Lemma concat_emp' :
-    forall n (t: n_tuple bool n), n_tuple_concat (tt: n_tuple _ 0) t = t.
+    forall n (t: n_tuple bool n), n_tuple_concat n_tuple_emp t = t.
   Proof.
     intros.
     apply JMeq_eq.
@@ -111,10 +119,10 @@ Section AutModel.
 
   Lemma interp_zero_tm:
      forall c (t: tm c (Bits 0)) v,
-       interp_tm (m := fm_model) v t = tt
-  .
+       interp_tm (m := fm_model) v t = n_tuple_emp.
   Proof.
-    intros; now destruct (interp_tm v t).
+    intros.
+    eapply n_tuple_emp_uniq.
   Qed.
 
 
@@ -122,7 +130,8 @@ Section AutModel.
     forall ctx srt (t : tm ctx srt) v,
       interp_tm (m := fm_model) v t = interp_tm v (simplify_concat_zero (ctx := ctx) t).
   Proof.
-    intros.
+  Admitted.
+    (* intros.
     dependent induction t using tm_ind'.
     - now autorewrite with simplify_concat_zero.
     - destruct srt;
@@ -144,7 +153,7 @@ Section AutModel.
         do 2 f_equal.
         apply H.
       + now autorewrite with simplify_concat_zero.
-  Qed.
+  Qed. *)
 
   Equations simplify_concat_zero_fm {ctx} (e: fm ctx) : fm ctx := {
     simplify_concat_zero_fm FTrue := FTrue;
@@ -162,7 +171,8 @@ Section AutModel.
       interp_fm valu f <-> interp_fm (m := fm_model) valu (simplify_concat_zero_fm f)
   .
   Proof.
-    intros.
+  Admitted.
+    (* intros.
     induction f; autorewrite with simplify_concat_zero_fm;
     (try now split; intros; auto);
     autorewrite with interp_fm;
@@ -173,7 +183,7 @@ Section AutModel.
     - erewrite IHf1. erewrite IHf2. split; intros; auto.
     - erewrite IHf1. erewrite IHf2. split; intros; auto.
     - setoid_rewrite IHf. split; intros; auto.
-  Qed.
+  Qed. *)
 
   Equations simplify_eq_zero_fm {ctx} (e: fm ctx) : fm ctx := {
     simplify_eq_zero_fm FTrue := FTrue;
@@ -185,7 +195,6 @@ Section AutModel.
     simplify_eq_zero_fm (FImpl f1 f2) := FImpl (simplify_eq_zero_fm f1) (simplify_eq_zero_fm f2);
     simplify_eq_zero_fm (FForall f) := FForall _ (simplify_eq_zero_fm f);
   }.
-
   Next Obligation.
   destruct e0 eqn:?.
   - destruct n.
@@ -198,7 +207,8 @@ Section AutModel.
     forall ctx (f: fm ctx) valu,
       interp_fm valu f <-> interp_fm (m := fm_model) valu (simplify_eq_zero_fm f).
   Proof.
-    intros.
+  Admitted.
+    (* intros.
     induction f; autorewrite with simplify_eq_zero_fm;
     (try now split; intros; auto);
     autorewrite with interp_fm;
@@ -214,7 +224,7 @@ Section AutModel.
     - erewrite IHf1. erewrite IHf2. split; intros; auto.
     - erewrite IHf1. erewrite IHf2. split; intros; auto.
     - setoid_rewrite IHf. split; intros; auto.
-  Qed.
+  Qed. *)
 
 
   (* It feels like this should be an instance of map_subst, but I can't get
@@ -228,7 +238,6 @@ Section AutModel.
   Qed.
 
 End AutModel.
-
 
 Register TVar as p4a.core.var.
 Register TFun as p4a.core.fun.
@@ -251,12 +260,8 @@ Register FImpl as p4a.core.impl.
 Register CEmp as p4a.core.cnil.
 Register CSnoc as p4a.core.csnoc.
 
-(* Register FirstOrderConfRelSimplified.Bits as p4a.sorts.bits. *)
 Register FirstOrderConfRelSimplified.Store as p4a.sorts.store.
 
-(* Register FirstOrderConfRelSimplified.BitsLit as p4a.funs.bitslit. *)
-(* Register FirstOrderConfRelSimplified.Concat as p4a.funs.concat. *)
-(* Register FirstOrderConfRelSimplified.Slice as p4a.funs.slice. *)
 Register FirstOrderConfRelSimplified.Lookup as p4a.funs.lookup.
 
 Register HList.HNil as p4a.core.hnil.
